semantics.v
@@ -12,7 +12,7 @@ Inductive decompose : term -> ctxt -> term -> Prop :=
 |appHole : forall e v, value v -> decompose (app (lambda e) v) hole (app (lambda e) v)
 |decompGet : forall e E e', decompose e E e' -> 
                             decompose (get e) (getCtxt E) e'
-|decompGetHole : forall l, decompose (get (loc l)) hole (get (loc l))
+|decompGetHole : forall l, decompose (get (loc l)) hole (get (loc l)) 
 |decompPut : forall e1 e2 E e, decompose e1 E e -> 
                                decompose (put e1 e2) (putCtxt e2 E) e
 |decompPutVal : forall v e2 E e (prf:value v), 
@@ -97,22 +97,21 @@ Inductive validateRes : Type :=
 |abort : term -> log -> validateRes. 
 
 (*Transactional log validation*)
-Inductive validate : stamp -> log -> heap -> stamp -> validateRes -> Prop :=
-|validateNil : forall S S' H, validate S nil H S' (commit H)
-|validateCommitRead : forall S S' S'' l v E H H' L,
-                        lookup H l = Some(v, S') -> S > S' -> 
-                        validate S L H S'' (commit H') ->
-                        validate S (readItem l E v::L) H S'' (commit H')
-|validateAbortPropogate : forall S S' L H x L' e, 
-                            validate S L H S' (abort e L') ->
-                            validate S (x::L) H S' (abort e L')
-|validateAbortRead : forall S S' S'' H L E H' l v v',
-              validate S L H S'' (commit H') -> lookup H l = Some(v, S') ->
-              S' > S -> validate S (readItem l E v'::L) H S'' 
-                                (abort (fill E(get(loc l))) L)
-|validateWrite : forall S S' L H H' l v,
-                   validate S L H S' (commit H') ->
-                   validate S (writeItem l v::L) H S' (commit ((l, v, S')::H'))
+Inductive validate : log -> heap -> validateRes -> Prop :=
+|validateNil : forall H, validate nil H (commit H)
+|validateCommitRead : forall l v E H H' L,
+                        H l = Some v -> 
+                        validate L H (commit H') ->
+                        validate (readItem l E v::L) H (commit H')
+|validateAbortPropogate : forall L H x L' e, 
+                            validate L H (abort e L') ->
+                            validate (x::L) H (abort e L')
+|validateAbortRead : forall H L E H' l v v',
+              validate L H (commit H') -> H l = Some v' -> v <> v' ->
+              validate (readItem l E v::L) H (abort (fill E(get(loc l))) L)
+|validateWrite : forall L H H' l v,
+                   validate L H (commit H') ->
+                   validate (writeItem l v::L) H (commit (update H' l v))
 .
 
 (*lookup a term in a thread's write set*)
@@ -143,160 +142,131 @@ Fixpoint open (e:term) (k:nat) (e':term) :=
   end. 
 
 (*transactional step (used by both p_step and f_step)*) 
-Inductive trans_step (H:heap) : thread -> thread -> Prop :=
-|t_readStep : forall S L E l t v e0 S', 
-                decompose t E (get (loc l)) -> logLookup L l = None ->
-                lookup H l = Some(v, S') -> S > S' ->
-                trans_step H (Some(S, e0), L, t) 
-                             (Some(S, e0), readItem l E v::L, fill E v)
+Inductive trans_step (H:heap) (C : nat) : thread -> thread -> Prop :=
+|t_readStep : forall L E l t v e0, 
+    decompose t E (get (loc l)) -> logLookup L l = None ->
+    H l = Some v -> 
+    trans_step H C (Some(C, e0), L, t) (Some(C, e0), readItem l E v::L, fill E v)
 |t_readInDomainStep : forall S l v L E t e0,
-                      decompose t E (get (loc l)) -> logLookup L l = Some v ->
-                      trans_step H (Some(S, e0), L, t) (Some(S, e0), L, fill E v)
+    decompose t E (get (loc l)) -> logLookup L l = Some v ->
+    trans_step H C (Some(S, e0), L, t) (Some(S, e0), L, fill E v)
 |t_writeStep : forall S L E l v t,
-               decompose t E (put (loc l) v) -> S <> None ->
-               trans_step H (S, L, t) (S, writeItem l v::L, fill E unit)
+    decompose t E (put (loc l) v) -> S <> None ->
+    trans_step H C (S, L, t) (S, writeItem l v::L, fill E unit)
 |t_atomicIdemStep : forall E e t L S,
-                     decompose t E (atomic e) -> S <> None ->
-                     trans_step H (S, L, t) (S, L, fill E e)
+    decompose t E (atomic e) -> S <> None ->
+    trans_step H C (S, L, t) (S, L, fill E e)
 |t_betaStep : forall L E e t v S, 
-              decompose t E (app (lambda e) v) -> S <> None ->
-              trans_step H (S, L, t) (S, L, fill E (open e 0 v))
+    decompose t E (app (lambda e) v) -> S <> None ->
+    trans_step H C (S, L, t) (S, L, fill E (open e 0 v))
 .
 
 (*same as trans_step with addition of r_readStepInvalid*)
-Inductive replay_step H : thread -> thread -> Prop :=
-|r_readStepValid : forall S L E l t v e0 S', 
-                lookup H l = Some(v, S') -> S > S' ->
-                decompose t E (get (loc l)) -> logLookup L l = None ->
-                replay_step H (Some(S, e0), L, t) (Some(S, e0), readItem l E v::L, fill E v)
-|r_readStepInvalid : forall S L E v' l t v e0 S', 
-                lookup H l = Some(v',S') -> S' >= S ->
-                decompose t E (get (loc l)) -> logLookup L l = None ->
-                replay_step H (Some(S, e0), L, t) (Some(S, e0), readItem l E v::L, fill E v)
+Inductive replay_step H (C : nat) : thread -> thread -> Prop :=
+|r_readStepValid : forall L E l t v e0, 
+    H l = Some v ->
+    decompose t E (get (loc l)) -> logLookup L l = None ->
+    replay_step H C (Some(C, e0), L, t) (Some(C, e0), readItem l E v::L, fill E v)
+|r_readStepInvalid : forall S L E v' l t v e0, 
+    H l = Some v' -> C > S ->
+    decompose t E (get (loc l)) -> logLookup L l = None ->
+    replay_step H C (Some(S, e0), L, t) (Some(S, e0), readItem l E v::L, fill E v)
 |r_readInDomainStep : forall S l v L E t e0,
-                      decompose t E (get (loc l)) -> logLookup L l = Some v ->
-                      replay_step H (Some(S, e0), L, t) (Some(S, e0), L, fill E v)
+    decompose t E (get (loc l)) -> logLookup L l = Some v ->
+    replay_step H C (Some(S, e0), L, t) (Some(S, e0), L, fill E v)
 |r_writeStep : forall S L E l v t,
-               decompose t E (put (loc l) v) -> S <> None ->
-               replay_step H (S, L, t) (S, writeItem l v::L, fill E unit)
+    decompose t E (put (loc l) v) -> S <> None ->
+    replay_step H C (S, L, t) (S, writeItem l v::L, fill E unit)
 |r_atomicIdemStep : forall E e t L S,
-                     decompose t E (atomic e) -> S <> None ->
-                     replay_step H (S, L, t) (S, L, fill E e)
+    decompose t E (atomic e) -> S <> None ->
+    replay_step H C (S, L, t) (S, L, fill E e)
 |r_betaStep : forall L E e t v S, 
-              decompose t E (app (lambda e) v) -> S <> None ->
-              replay_step H (S, L, t) (S, L, fill E (open e 0 v))
+    decompose t E (app (lambda e) v) -> S <> None ->
+    replay_step H C (S, L, t) (S, L, fill E (open e 0 v))
 .
 
 (*reflexive transitive closure of replay_step*)
-Inductive replay H : thread -> thread -> Prop :=
-|replayRefl : forall t, replay H t t
+Inductive replay H (C : nat) : thread -> thread -> Prop :=
+|replayRefl : forall t, replay H C t t
 |replayStep : forall t t' t'', 
-                replay_step H t t' -> replay H t' t'' -> 
-                replay H t t''. 
+                replay_step H C t t' -> replay H C t' t'' -> 
+                replay H C t t''. 
 
 (*left recursive version of replay*)
-Inductive rewind H : thread -> thread -> Prop :=
-|rewindRefl : forall t, rewind H t t
+Inductive rewind H (C : nat) : thread -> thread -> Prop :=
+|rewindRefl : forall t, rewind H C t t
 |rewindStep : forall t t' t'', 
-                rewind H t t' -> replay_step H t' t'' -> 
-                rewind H t t''. 
+                rewind H C t t' -> replay_step H C t' t'' -> 
+                rewind H C t t''. 
 
-(*parital abort STM semantics (single step)*)
-Inductive p_step : nat -> heap -> pool -> nat -> heap -> pool -> Prop :=
-|p_transStep : forall C H t t', trans_step H t t' -> 
-                           p_step C H (Single t) C H (Single t')
-|p_parLStep : forall C H T1 T2 C' H' T1', 
-          p_step C H T1 C' H' T1' -> p_step C H (Par T1 T2) C' H' (Par T1' T2)
-|p_parRStep : forall C H T1 T2 C' H' T2', 
-          p_step C H T2 C' H' T2' -> p_step C H (Par T1 T2) C' H' (Par T1 T2')
-|p_forkStep : forall C H E e t, 
+
+Definition step_sig := nat -> heap -> pool -> nat -> heap -> pool -> Prop. 
+
+Inductive c_step (st : step_sig) : step_sig :=
+|c_liftedStep : forall C H P C' H' P',
+                  st C H P C' H' P' ->
+                  c_step st C H P C' H' P'
+|c_transStep : forall C H t t',
+    trans_step H C t t' -> 
+    c_step st C H (Single t) C H (Single t')
+|c_parLStep : forall C H T1 T2 C' H' T1', 
+          c_step st C H T1 C' H' T1' -> c_step st C H (Par T1 T2) C' H' (Par T1' T2)
+|c_parRStep : forall C H T1 T2 C' H' T2', 
+          c_step st C H T2 C' H' T2' -> c_step st C H (Par T1 T2) C' H' (Par T1 T2')
+|c_forkStep : forall C H E e t, 
               decompose t E (fork e) ->
-              p_step C H (Single(None, nil, t)) C H 
-                   (Par (Single(None, nil, fill E unit)) (Single(None, nil, e)))
-|p_eagerAbort : forall L S H L' C e0 e' t v E l S',
-                  lookup H l = Some(v, S') -> S < S' ->
-                  validate S (readItem l E v::L) H C (abort e' L') ->
-                  decompose t E (get (loc l)) -> logLookup L l = None ->
-                  p_step C H (Single (Some(S, e0), L, t))
-                         (C+1) H (Single(Some(C, e0), L', e'))
-|p_abortStep : forall L S H L' C e e0 e' S', 
-           validate S L H S' (abort e' L') ->
-           p_step C H (Single(Some(S, e0), L, e))
-                  (plus 1 C) H (Single(Some(C, e0), L', e'))
-|p_allocStep : forall C H v E t l, 
-               lookup H l = None -> decompose t E (alloc v) ->
-               p_step C H (Single(None, nil, t)) (plus 1 C) ((l, v, C)::H)
-                    (Single(None, nil, fill E (loc l)))
-|p_commitStep : forall C H S L v t E H' e0, 
-                validate S L H C (commit H') -> decompose t E (inatomic v) ->
-                p_step C H (Single(Some(S, e0), L, t)) (plus 1 C) H' (Single(None, nil, fill E v))
-|p_atomicStep : forall C H E e t, 
+              c_step st C H (Single(None, nil, t)) C H 
+                   (Par (Single(None, nil, (fill E unit))) (Single(None, nil, e)))
+|c_allocStep : forall C H v E t l, 
+               H l = None -> decompose t E (alloc v) ->
+               c_step st C H (Single(None, nil, t)) C (update H l v)
+                    (Single(None, nil, (fill E (loc l))))
+|c_commitStep : forall C H HV S L v t E e0, 
+                  validate L H (commit HV) -> decompose t E (inatomic v) ->
+                  c_step st C H (Single(Some(S, e0), L, t)) (plus 1 C)
+                         HV (Single(None, nil, (fill E v)))
+|c_atomicStep : forall C H E e t, 
                 decompose t E (atomic e) ->
-                p_step C H (Single(None, nil, t)) (plus 1 C) H 
-                       (Single(Some(C, fill E(inatomic e)),[],fill E (inatomic e)))
-|p_betaStep : forall C H E e t v, 
+                c_step st C H (Single(None, nil, t)) C H 
+                       (Single(Some(C, fill E(inatomic e)), nil, (fill E (inatomic e))))
+|c_betaStep : forall C H E e t v, 
               decompose t E (app (lambda e) v) -> 
-              p_step C H (Single(None, nil, t)) C H
-                     (Single(None, nil, fill E (open e 0 v))). 
+              c_step st C H (Single(None, nil, t)) C H
+                     (Single(None, nil, (fill E (open e 0 v))))
+|c_tsExtend : forall C H t S L e0 HV,
+                validate L H (commit HV) ->
+                c_step st C H (Single(Some(S, e0), L, t)) C H
+                       (Single(Some(C, e0), L, t))
+.
 
-(*reflexive transitive closure of partial multistep*)
-Inductive p_multistep : nat -> heap -> pool -> nat -> heap -> pool -> Prop :=
-|p_multi_refl : forall C H T, p_multistep C H T C H T
-|p_multi_step : forall C H T C' H' T' C'' H'' T'', 
-                p_step C H T C' H' T' -> p_multistep C' H' T' C'' H'' T'' ->
-                p_multistep C H T C'' H'' T''. 
+Inductive p_step_ : step_sig :=
+|p_abort : forall C H S L L' e' e e0,
+    validate L H (abort e' L') ->
+    p_step_ C H (Single(Some(S, e0), L, e)) C H (Single(Some(C, e0), L', e')). 
 
-(*full abort STM semantics (single step)*)
-Inductive f_step : nat -> heap -> pool -> nat -> heap -> pool -> Prop :=
-|f_transStep : forall C H t t', trans_step H t t' -> 
-                           f_step C H (Single t) C H (Single t')
-|f_parLStep : forall C H T1 T2 C' H' T1', 
-          f_step C H T1 C' H' T1' -> f_step C H (Par T1 T2) C' H' (Par T1' T2)
-|f_parRStep : forall C H T1 T2 C' H' T2', 
-          f_step C H T2 C' H' T2' -> f_step C H (Par T1 T2) C' H' (Par T1 T2')
-|f_forkStep : forall C H E e t, 
-              decompose t E (fork e) ->
-              f_step C H (Single(None, nil, t)) C H 
-                   (Par (Single(None, nil, fill E unit)) (Single(None, nil, e)))
-|f_eagerAbort : forall L S H L' C e0 e' t v E l S',
-                  lookup H l = Some(v, S') -> S < S' ->
-                  validate S (readItem l E v::L) H C (abort e' L') ->
-                  decompose t E (get (loc l)) -> logLookup L l = None ->
-                  f_step C H (Single (Some(S, e0), L, t))
-                         (C+1) H (Single(Some(C, e0), nil, e0))
-|f_abortStep : forall L S H L' C e e0 e' S', 
-           validate S L H S' (abort e' L') -> 
-           f_step C H (Single(Some(S, e0), L, e)) (plus 1 C) H 
-                  (Single(Some(C, e0), nil, e0))
-|f_allocStep : forall C H v E t l, 
-               lookup H l = None -> decompose t E (alloc v) ->
-               f_step C H (Single(None, nil, t)) (plus 1 C) ((l, v, C)::H)
-                    (Single(None, nil, fill E (loc l)))
-|f_commitStep : forall C H S L v t E H' e0, 
-                validate S L H C (commit H') -> decompose t E (inatomic v) ->
-                f_step C H (Single(Some(S, e0), L, t)) (plus 1 C) H' (Single(None, nil, fill E v))
-|f_atomicStep : forall C H E e t, 
-                decompose t E (atomic e) ->
-                f_step C H (Single(None, nil, t)) (plus 1 C) H 
-                       (Single(Some(C, fill E (inatomic e)), nil, fill E (inatomic e)))
-|f_betaStep : forall C H E e t v, 
-              decompose t E (app (lambda e) v) -> 
-              f_step C H (Single(None, nil, t)) C H 
-                     (Single(None, nil, fill E (open e 0 v))). 
+Inductive f_step_ : step_sig :=
+|f_abort : forall C H S L L' e' e e0,
+    validate L H (abort e' L') ->
+    f_step_ C H (Single(Some(S, e0), L, e)) C H (Single(Some(C, e0), nil, e0)). 
 
-(*reflexivie transitive closure of full multistep*)
-Inductive f_multistep : nat -> heap -> pool -> nat -> heap -> pool -> Prop :=
-|f_multi_refl : forall C H T, f_multistep C H T C H T
-|f_multi_step : forall C H T C' H' T' C'' H'' T'', 
-                f_step C H T C' H' T' -> f_multistep C' H' T' C'' H'' T'' ->
-                f_multistep C H T C'' H'' T''. 
+                   
+Inductive c_multistep (st : step_sig) : step_sig :=
+  c_multi_refl : forall C H T, c_multistep st C H T C H T
+| c_multi_step : forall C H T C' H' T' C'' H'' T'',
+    c_step st C H T C' H' T' -> c_multistep st C' H' T' C'' H'' T'' ->
+    c_multistep st C H T C'' H'' T''. 
 
-(*reflexivit transitive closure of trans_step*)
-Inductive trans_multistep H : thread -> thread -> Prop :=
-|trans_refl : forall t, trans_multistep H t t
+Definition p_step := c_step p_step_.
+Definition f_step := c_step f_step_. 
+Definition p_multistep := c_multistep p_step.
+Definition f_multistep := c_multistep f_step.  
+
+(*reflexivie transitive closure of trans_step*)
+Inductive trans_multistep H C : thread -> thread -> Prop :=
+|trans_refl : forall t, trans_multistep H C t t
 |trans_multi_step : forall t t' t'', 
-                      trans_step H t t' -> trans_multistep H t' t'' ->
-                      trans_multistep H t t''. 
+                      trans_step H C t t' -> trans_multistep H C t' t'' ->
+                      trans_multistep H C t t''. 
 
 (*indicates that L1 is a postfix of L2*)
 Definition postfix {A:Type} (L1 L2 : list A) := exists diff, L2 = diff ++ L1. 
@@ -307,8 +277,8 @@ Definition postfix {A:Type} (L1 L2 : list A) := exists diff, L2 = diff ++ L1.
 Inductive poolRewind C H : pool -> Prop :=
 |rewindSingleNoTX : forall e, poolRewind C H (Single(None,nil,e))
 |rewindSingleInTX : forall S e0 L e, 
-                      rewind H (Some(S,e0),nil,e0) (Some(S,e0),L,e) ->
-                      S < C -> poolRewind C H (Single(Some(S,e0),L,e))
+                      rewind H C (Some(S,e0),nil,e0) (Some(S,e0),L,e) ->
+                      S <= C -> poolRewind C H (Single(Some(S,e0),L,e))
 |rewindPar : forall T1 T2, poolRewind C H T1 -> poolRewind C H T2 -> poolRewind C H (Par T1 T2). 
 
 (*inject every step in a multistep derivation into a Par*)
@@ -318,7 +288,7 @@ Theorem f_multi_L : forall C H T1 T2 T1' C' H',
 Proof.
   intros C H T1 T2 T1' C' H' HYP. induction HYP.
   {constructor. }
-  {econstructor. eapply f_parLStep. eassumption. eassumption. }
+  {econstructor. eapply c_parLStep. eassumption. eassumption. }
 Qed. 
 
 (*inject every step in a multistep derivation into a Par*)
@@ -328,25 +298,25 @@ Theorem f_multi_R : forall C H T1 T2 T2' C' H',
 Proof.
   intros C H T1 T2 T2' C' H' HYP. induction HYP.
   {constructor. }
-  {econstructor. eapply f_parRStep. eassumption. eassumption. }
+  {econstructor. eapply c_parRStep. eassumption. eassumption. }
 Qed. 
 
 (*validation is idempotent*)
-Theorem validateValidate : forall S L H S' L' e, 
-                             validate S L H S' (abort e L') ->
-                             exists H'', validate S L' H S' (commit H''). 
+Theorem validateValidate : forall L H L' e, 
+                             validate L H (abort e L') ->
+                             exists H'', validate L' H (commit H''). 
 Proof.
-  intros S L H S' L' e HYP. dependent induction HYP; eauto. 
+  intros L H L' e HYP. dependent induction HYP; eauto. 
 Qed. 
 
 (*the log returned in an abort is a postfix of the initial log*)
-Theorem abortLogPostfix : forall S L H S' L' e, 
-                            validate S L H S' (abort e L') ->
+Theorem abortLogPostfix : forall L H L' e, 
+                            validate L H (abort e L') ->
                             postfix L' L. 
 Proof.
-  intros S L H S' L' e HYP. remember (abort e L'). induction HYP; try solveByInv. 
+  intros L H L' e HYP. remember (abort e L'). induction HYP; try solveByInv. 
   {apply IHHYP in Heqv. unfold postfix in *. invertHyp.  exists (x::x0). auto. }
-  {inv Heqv. unfold postfix. exists [readItem l E v']. auto. }
+  {inv Heqv. unfold postfix. exists [readItem l E v]. simpl. auto. }
 Qed.
 
 (*filling an evaluation context with the result of a decomposition
@@ -365,27 +335,27 @@ Proof.
 Qed. 
 
 (*replay relation is transitive*)
-Theorem trans_replay: forall H t t' t'', 
-                         replay H t' t'' -> replay H t t' ->
-                         replay H t t''. 
+Theorem trans_replay: forall H t t' t'' C, 
+                         replay H C t' t'' -> replay H C t t' ->
+                         replay H C t t''. 
 Proof.
-  intros H t t' t'' HYP1 HYP2. induction HYP2. auto. econstructor. eauto. auto. 
+  intros H t t' t'' C HYP1 HYP2. induction HYP2. auto. econstructor. eauto. auto. 
 Qed. 
 
 (*rewind relation is transitive*)
-Theorem rewindTrans : forall H t t' t'', 
-                        rewind H t t' -> rewind H t' t'' ->
-                        rewind H t t''. 
+Theorem rewindTrans : forall C H t t' t'', 
+                        rewind H C t t' -> rewind H C t' t'' ->
+                        rewind H C t t''. 
 Proof.
-  intros H t t' t'' HYP1 HYP2. generalize dependent t. induction HYP2; intros; auto.
+  intros C H t t' t'' HYP1 HYP2. generalize dependent t. induction HYP2; intros; auto.
   econstructor. eapply IHHYP2. assumption. assumption. 
 Qed. 
 
 (*replay and rewind are equivalent*)
-Theorem rewindIFFReplay : forall H t t', 
-                            rewind H t t' <-> replay H t t'. 
+Theorem rewindIFFReplay : forall H t t' C, 
+                            rewind H C t t' <-> replay H C t t'. 
 Proof.
-  intros H t t'. split; intros HYP. 
+  intros. split; intros HYP. 
   {induction HYP. constructor. eapply trans_replay; eauto.
    econstructor. eauto. constructor. }
   {induction HYP. constructor. eapply rewindTrans; eauto.
@@ -393,41 +363,32 @@ Proof.
 Qed. 
 
 (*partial multistep relation is transitive*)
-Theorem p_multi_trans : forall C H T C' H' T' C'' H'' T'',
-                          p_multistep C H T C' H' T' ->
-                          p_multistep C' H' T' C'' H'' T'' ->
-                          p_multistep C H T C'' H'' T''.
+Theorem c_multi_trans : forall st C H T C' H' T' C'' H'' T'',
+                          c_multistep st C H T C' H' T' ->
+                          c_multistep st C' H' T' C'' H'' T'' ->
+                          c_multistep st C H T C'' H'' T''.
 Proof.
-  intros C H T C' H' T' C'' H'' T'' HYP1 HYP2. 
-  induction HYP1; auto. econstructor; eauto.
-Qed. 
-
-(*full multistep relation is transitive*)
-Theorem f_multi_trans : forall C H T C' H' T' C'' H'' T'',
-                          f_multistep C H T C' H' T' ->
-                          f_multistep C' H' T' C'' H'' T'' ->
-                          f_multistep C H T C'' H'' T''.
-Proof.
-  intros C H T C' H' T' C'' H'' T'' HYP1 HYP2. 
-  induction HYP1; auto. econstructor; eauto. 
-Qed. 
+  intros. induction H0.
+  {auto. }
+  {econstructor; eauto. }
+Qed.
 
 (*inject left multistep derivation into a Par*)
-Theorem p_multi_L : forall C H T1 T2 T1' C' H', 
-                      p_multistep C H T1 C' H' T1' ->
-                      p_multistep C H (Par T1 T2) C' H' (Par T1' T2). 
+Theorem c_multi_L : forall st C H T1 T2 T1' C' H', 
+                      c_multistep st C H T1 C' H' T1' ->
+                      c_multistep st C H (Par T1 T2) C' H' (Par T1' T2). 
 Proof.
   intros. induction H0.
   {constructor. }
-  {econstructor. eapply p_parLStep. eassumption. eassumption. }
+  {econstructor. eapply c_parLStep. eassumption. eauto. }
 Qed. 
 
 (*inject right multistep derivation into a Par*)
-Theorem p_multi_R : forall C H T1 T2 T2' C' H', 
-                      p_multistep C H T2 C' H' T2' ->
-                      p_multistep C H (Par T1 T2) C' H' (Par T1 T2'). 
+Theorem c_multi_R : forall st C H T1 T2 T2' C' H', 
+                      c_multistep st C H T2 C' H' T2' ->
+                      c_multistep st C H (Par T1 T2) C' H' (Par T1 T2'). 
 Proof.
   intros. induction H0.
   {constructor. }
-  {econstructor. eapply p_parRStep. eassumption. eassumption. }
+  {econstructor. eapply c_parRStep. eassumption. eassumption. }
 Qed. 
