stepPreservesRewind.v
@@ -1,196 +1,108 @@
 Require Export semantics. 
 
-(*retrieve the stamp number from a heap location*)
-Definition getStamp (x : location * term * stamp) :=
-  match x with
-      |(_,_,s) => s
-  end.  
-
-(*if location l is present in heap H, then if we extend H with some number of
-**locations, all of which have stamp C.  Then either we will get the same 
-**result when looking up in the extended heap or we will get something that 
-**has a timestamp of C*)
-Theorem lookupExtension : forall H' l v S H C, 
-                  lookup H l = Some(v, S) ->
-                  Forall (fun x : location * term * stamp => getStamp x = C) H' ->
-                  lookup (H'++H) l = Some(v, S) \/
-                  exists S' v', lookup (H'++H) l = Some(v', S') /\
-                           S' = C. 
+Theorem rewindAllocSingle : forall v C H S e0 L e L' e' l,
+    rewind H C (Some(S, e0), L, e) (Some(S, e0), L', e') ->
+    H l = None ->
+    rewind (update H l v) C (Some(S, e0), L, e) (Some(S, e0), L', e'). 
 Proof.
-  induction H'; intros l v S H C HYP1 HYP2. 
-  {simpl. auto. }
-  {simpl in *. destruct a. destruct p. destruct (eq_nat_dec l l0). 
-   {right. subst. repeat econstructor. inv HYP2. auto. }
-   {inv HYP2. eapply IHH' in HYP1; eauto. }
-  }
-Qed. 
-
-(*we can produce the same replay derivation under an extended heap, if everything
-**in the extension has a timestamp greater than the thread being replayed*)
-Theorem replayHeapExtension : forall H H' S e0 L e L' e' C,
-                      replay H (Some(S,e0),L,e) (Some(S,e0),L',e') -> S < C ->
-                      Forall (fun x : location * term * stamp => getStamp x = C) H' ->
-                      replay (H'++H) (Some(S,e0),L,e) (Some(S,e0),L',e'). 
-Proof.
-  intros. dependent induction H0. 
-  {constructor. }
-  {inv H0. 
-   {copy H8. eapply lookupExtension with (H':=H') in H0; eauto. inv H0. 
-    {econstructor. eapply r_readStepValid; eauto. eauto. }
-    {invertHyp. econstructor. eapply r_readStepInvalid; eauto. omega. eauto. }
+  intros. dependent induction H0.
+  {econstructor. }
+  {inv H1.
+   {econstructor; eauto. econstructor; eauto.
+    unfold update. destruct (Nat.eq_dec l l0).
+    {subst. transEq. invertEq. }
+    {assumption. }
    }
-   {copy H8. eapply lookupExtension with (H':=H') in H0; eauto. inv H0. 
-    {econstructor. eapply r_readStepInvalid; eauto. eauto. }
-    {invertHyp. econstructor. eapply r_readStepInvalid; eauto. omega. eauto. }
+   {econstructor; eauto. econstructor; eauto.
+    unfold update. destruct (Nat.eq_dec l l0).
+    {subst. transEq. invertEq. }
+    {eassumption. }
    }
-   {econstructor. eapply r_readInDomainStep; eauto. eauto. }
-   {econstructor. eapply r_writeStep; eauto. eauto. }
-   {econstructor. eapply r_atomicIdemStep; eauto. eauto. }
-   {econstructor. eapply r_betaStep; eauto. eauto. }
+   {econstructor; eauto. econstructor; eauto. }
+   {econstructor; eauto. econstructor; eauto. }
+   {econstructor; eauto. eapply r_atomicIdemStep; eauto. }
+   {econstructor; eauto. eapply r_betaStep; eauto. }
   }
-Qed. 
+Qed.
 
-(*Generalizes the previous theorem to thread pools*)
-Theorem poolRewindHeapExtension : forall H H' T C C', 
-                                    C' >= C -> poolRewind C H T ->
-                                    Forall (fun x : location * term * stamp => getStamp x = C) H' ->
-                                    poolRewind C' (H'++H) T.
-Proof.
-  intros. induction H1. 
-  {constructor. }
-  {constructor. rewrite rewindIFFReplay. eapply replayHeapExtension; eauto. 
-   rewrite <- rewindIFFReplay. auto. omega. }
-  {constructor; auto. }
-Qed. 
-
-
-(*If the log at the end of a rewind derivation is invalid, then we can rewind
-**from the log returned from validate*)
-Theorem abortRewind : forall S L H S' e' L' e0 e,
-                        validate S L H S' (abort e' L') ->
-                        rewind H (Some (S, e0), [], e0) (Some (S, e0), L, e) ->
-                        rewind H (Some (S, e0), [], e0) (Some (S, e0), L', e'). 
-Proof.
-  intros. dependent induction H1. 
-  {inv H0. }
-  {inv H2; eauto. 
-   {inv H0; eauto. apply decomposeEq in H10. subst. auto. }
-   {inv H0; eauto. eapply decomposeEq in H10. subst. auto. }
-   {inv H0. eauto. }
-  }
-Qed. 
-
-Ltac lookupSame :=
-  match goal with
-      |H:logLookup ?L ?l = ?v, H':logLookup ?L ?l = ?v' |- _ =>
-       rewrite H in H'; inv H'
-      |A:lookup ?H ?l = ?v, B:lookup ?H ?l = ?v' |- _ =>
-       rewrite A in B; inv B
-  end. 
-
-(*the same rewind derivation can be produced with a newer stamp assuming the 
-**log is valid*)
-Theorem rewindDiffStamp : forall S C H e0 L e L' e' H' S', 
-                        rewind H (Some(S,e0), L, e) (Some(S,e0), L', e') -> C > S ->
-                        validate S L' H S' (commit H') ->
-                        rewind H (Some(C,e0), L, e) (Some(C,e0), L', e').
-Proof.
-  intros. generalize dependent H'. dependent induction H0; intros. constructor. 
-  inv H1.
-  {econstructor. Focus 2. eapply r_readStepValid; eauto. omega.  
-   eapply IHrewind; eauto. inv H3. eauto. }
-  {inv H3. lookupSame. omega. }
-  {econstructor. Focus 2. eapply r_readInDomainStep; eauto. eauto. }
-  {inv H3. econstructor. Focus 2. eapply r_writeStep; eauto. intros c. inv c. 
-   eapply IHrewind; eauto. }
-  {econstructor. Focus 2. eapply r_atomicIdemStep; eauto. intros c. inv c. eauto. }
-  {econstructor. Focus 2. eapply r_betaStep; eauto. intros c. inv c. eauto. }
-Qed. 
-
-(*rewind can always take place on a newer timestamp*)
-Theorem poolRewindWeakening : forall C C' H T,
-                                poolRewind C H T -> C' >= C ->
-                                poolRewind C' H T. 
+Theorem rewindAlloc : forall v C H T l,
+    poolRewind C H T -> H l = None ->
+    poolRewind C (update H l v) T. 
 Proof.
   intros. induction H0.
+  {econstructor. }
+  {econstructor; auto. eapply rewindAllocSingle; auto. }
+  {econstructor; eauto. }
+Qed. 
+
+Theorem commitLookup : forall L H HV l v,
+    H l = Some v -> validate L H (commit HV) ->
+    exists v', HV l = Some v'.
+Proof.
+  intros. dependent induction H1; eauto. unfold update.
+  destruct (Nat.eq_dec l0 l); eauto.
+Qed. 
+
+  
+Theorem rewindCommitSingleNI : forall C H S e0 L e L' e' HV L'',
+    validate L'' H (commit HV) -> S <= C ->
+    rewind H C (Some(S, e0), L, e) (Some(S, e0), L', e') ->
+    rewind HV (1+C) (Some(S, e0), L, e) (Some(S, e0), L', e'). 
+Proof.
+  intros. genDeps{{HV; L''}}. dependent induction H2; intros.
+  {econstructor. }
+  {inv H3.
+   {econstructor. eapply IHrewind; eauto.
+    eapply commitLookup in H0; eauto. invertHyp.
+    eapply r_readStepInvalid; eauto. }
+   {econstructor. eapply IHrewind; eauto. eapply commitLookup in H0; eauto.
+    invertHyp. eapply r_readStepInvalid; eauto. }
+   {econstructor. eapply IHrewind; eauto. econstructor; eauto. }
+   {econstructor. eapply IHrewind; eauto. econstructor; eauto. }
+   {econstructor. eapply IHrewind; eauto. eapply r_atomicIdemStep; eauto. }
+   {econstructor. eapply IHrewind; eauto. eapply r_betaStep; eauto. }
+  }
+Qed. 
+    
+Theorem rewindCommitNI : forall C H T HV L,
+    validate L H (commit HV) ->
+    poolRewind C H T -> poolRewind (1+C) HV T. 
+Proof.
+  intros. induction H1.
+  {repeat econstructor. }
+  {econstructor; auto. eapply rewindCommitSingleNI; eauto. }
+  {econstructor; eauto. }
+Qed. 
+  
+Theorem f_stepNI : forall C H T1 C' H' T1' T2,
+       f_step C H T1 C' H' T1' -> poolRewind C H T2 ->
+       poolRewind C' H' T2. 
+Proof.
+  intros. induction H0; auto. 
+  {inv H0. auto. }
+  {eapply rewindAlloc; eauto. }
+  {eapply rewindCommitNI; eauto. }
+Qed.
+
+Theorem rewindNewerStamp : forall H C S e0 e e' L L' HV,
+    validate L' H (commit HV) ->
+    rewind H C (Some(S, e0), L, e) (Some(S, e0), L', e') ->
+    rewind H C (Some(C, e0), L, e) (Some(C, e0), L', e'). 
+Proof.
+  intros. generalize dependent HV. dependent induction H1; intros. 
   {constructor. }
-  {constructor; auto. omega. }
-  {constructor; auto. }
-Qed. 
-
-(*if a heap can be validated, then the resulting heap is an extension of the 
-**input heap*)
-Theorem validateHeapExtension : forall S H C H' L,
-                                    validate S L H C (commit H')  ->
-                                    exists H'', H' = H'' ++ H .
-Proof.
-  intros. dependent induction H0; eauto; try solve[exists nil; eauto].  
-  {invertHyp. exists ((l,v,S')::x). simpl. reflexivity. }
-Qed. 
-
-(*when validating the heap, the extended portion must all have time stamp
-**equal to the write version number*)
-Theorem validateStampGE : forall H' S L H C,
-                            validate S L H C (commit (H'++H)) ->
-                            Forall (fun x => getStamp x = C) H'. 
-Proof.
-  intros. dependent induction H0; auto. 
-  {destruct H'. constructor. apply lengthsEq in x. simpl in *. 
-   rewrite app_length in x. omega. }
-  {copy H0. eapply validateHeapExtension in H0. invertHyp. destruct H'. 
-   simpl in x. apply lengthsEq in x. simpl in x. rewrite app_length in x. omega.
-   constructor. inv x. auto. eapply IHvalidate; eauto. inversion x. auto. }
-Qed. 
-
-(*version clock and heap increase monotonically under the p_step relation*)
-Theorem p_stampHeapMonotonic : forall C H T C' H' T',
-             p_step C H T C' H' T' -> 
-             C' >= C /\ (exists H'', H' = H'' ++ H /\ Forall (fun x => getStamp x = C) H''). 
-Proof.
-  intros. induction H0; try invertHyp; split; eauto; try solve[exists nil; auto]. omega.  
-  {exists [(l,v,C)]. simpl. split; auto.  }
-  {copy H0. apply validateHeapExtension in H0. invertHyp. exists x. split; auto. 
-   eapply validateStampGE in H2. auto. }
-Qed. 
-
-(*p_step preserves rewind*)
-Theorem p_stepRewind : forall C H T C' H' T', 
-                       p_step C H T C' H' T' -> poolRewind C H T ->
-                       poolRewind C' H' T'. 
-Proof.
-  intros. induction H0; try solve[repeat econstructor]. 
-  {inv H1. inv H0; exfalso; apply H6; auto. inv H0. 
-   {destruct(lt_dec S' S). 
-    {constructor; auto. econstructor; eauto. eapply r_readStepValid; eauto. }
-    {constructor; auto. econstructor; eauto. eapply r_readStepInvalid; eauto. omega. }
-   }
-   {constructor. econstructor; eauto. eapply r_readInDomainStep; eauto. auto. }
-   {econstructor. econstructor; eauto. eapply r_writeStep; eauto. auto. }
-   {econstructor. econstructor; eauto. eapply r_atomicIdemStep; eauto. auto. }
-   {econstructor. econstructor; eauto. eapply r_betaStep; eauto. auto. }
+  {inv H2.
+   {econstructor. eassumption. econstructor; auto. }
+   {inv H0. transEq. invertEq. econstructor. eapply IHrewind; eauto. 
+    econstructor; eauto. }
+   {econstructor. eapply IHrewind; eauto. econstructor; eauto. }
+   {inv H0. econstructor. eapply IHrewind; eauto.
+    econstructor; eauto. intro. solveByInv. }
+   {econstructor. eapply IHrewind; eauto.
+    eapply r_atomicIdemStep; eauto. intro. solveByInv. }
+   {econstructor. eapply IHrewind; eauto.
+    eapply r_betaStep; eauto. intro. solveByInv. }
   }
-  {inv H1. constructor; auto. eapply p_stampHeapMonotonic in H0. invertHyp. 
-   eapply poolRewindHeapExtension; eauto. }
-  {inv H1. constructor; auto.  eapply p_stampHeapMonotonic in H0. invertHyp. 
-   eapply poolRewindHeapExtension; eauto. }
-  {inv H1. constructor; try omega. inv H3. 
-   {copy H13. eapply abortRewind in H13; eauto. eapply validateValidate in H1. 
-    invertHyp. eapply rewindDiffStamp; eauto. }
-   {apply decomposeEq in H4. subst. eapply rewindDiffStamp; eauto. }
-  }
-  {inv H1. econstructor; try omega. copy H0. eapply abortRewind in H0; eauto.
-   eapply validateValidate in H1; eauto. invertHyp. eapply rewindDiffStamp; eauto. }
-Qed. 
-
-(*version clock and heap increase monotonically under the f_step relation*)
-Theorem f_stampHeapMonotonic : forall C H T C' H' T',
-                               f_step C H T C' H' T' -> 
-                               C' >= C /\ (exists H'', H' = H'' ++ H /\ Forall (fun x => getStamp x = C) H''). 
-Proof.
-  intros. induction H0; try invertHyp; split; eauto; try solve[exists nil; auto]. omega.  
-  {exists [(l,v,C)]. simpl. split; auto.  }
-  {copy H0. apply validateHeapExtension in H0. invertHyp. exists x. split; auto. 
-   eapply validateStampGE in H2. auto. }
 Qed. 
 
 (*f_step preserves rewind*)
@@ -198,20 +110,82 @@ Theorem f_stepRewind : forall C H T C' H' T',
                        f_step C H T C' H' T' -> poolRewind C H T ->
                        poolRewind C' H' T'. 
 Proof.
-  intros. induction H0; try solve[repeat econstructor]. 
-  {inv H1. inv H0; exfalso; apply H6; auto. inv H0. 
-   {destruct(lt_dec S' S). 
-    {constructor; auto. econstructor; eauto. eapply r_readStepValid; eauto. }
-    {constructor; auto. econstructor; eauto. eapply r_readStepInvalid; eauto. omega. }
-   }
-   {constructor. econstructor; eauto. eapply r_readInDomainStep; eauto. auto. }
-   {econstructor. econstructor; eauto. eapply r_writeStep; eauto. auto. }
-   {econstructor. econstructor; eauto. eapply r_atomicIdemStep; eauto. auto. }
-   {econstructor. econstructor; eauto. eapply r_betaStep; eauto. auto. }
+  intros. induction H0. 
+  {inv H0. econstructor; auto. econstructor. }
+  {inv H0.
+   {inv H1. econstructor; auto. econstructor. 
+    eassumption. econstructor; eauto. }
+   {inv H1. econstructor; auto. econstructor. eassumption.
+    econstructor; eauto. }
+   {inv H1. exfalso; auto. econstructor; eauto.
+    econstructor. eassumption. econstructor; eauto. }
+   {inv H1. exfalso; auto. econstructor; auto.
+    econstructor. eassumption. eapply r_atomicIdemStep; eauto. }
+   {inv H1. exfalso; auto. econstructor; auto.
+    econstructor. eassumption. eapply r_betaStep; eauto. }
   }
-  {inv H1. constructor; auto. eapply f_stampHeapMonotonic in H0. 
-   invertHyp. eapply poolRewindHeapExtension; eauto. }
-  {inv H1. constructor; auto. eapply f_stampHeapMonotonic in H0. 
-   invertHyp. eapply poolRewindHeapExtension; eauto. }
-  {constructor. constructor. omega. }
+  {inv H1. econstructor; eauto. eapply f_stepNI; eauto. }
+  {inv H1. econstructor; eauto. eapply f_stepNI; eauto. }
+  {repeat econstructor. }
+  {repeat econstructor. }
+  {econstructor. }
+  {econstructor. econstructor. auto. }
+  {econstructor. }
+  {inv H1. econstructor; auto. eapply rewindNewerStamp; eauto. }
+Qed. 
+
+Theorem p_stepNI : forall C H T1 C' H' T1' T2,
+       p_step C H T1 C' H' T1' -> poolRewind C H T2 ->
+       poolRewind C' H' T2. 
+Proof.
+  intros. induction H0; auto. 
+  {inv H0. auto. }
+  {eapply rewindAlloc; eauto. }
+  {eapply rewindCommitNI; eauto. }
+Qed.
+
+Theorem rewindAbort : forall H C S e0 L' e' L'' e'',
+    validate L' H (abort e'' L'') ->
+    rewind H C (Some(S, e0), nil, e0) (Some(S, e0), L', e') ->
+    rewind H C (Some(S, e0), nil, e0) (Some(S, e0), L'', e'').
+Proof.
+  intros. genDeps{{L''; e''}}. dependent induction H1; intros.
+  {inv H0. }
+  {inv H2; eauto. 
+   {inv H0; eauto. eapply decomposeEq in H9.
+    subst. assumption. }
+   {inv H0; eauto. eapply decomposeEq in H10. subst. eauto. }
+   {inv H0. eauto. }
+  }
+Qed. 
+  
+(*p_step preserves rewind*)
+Theorem p_stepRewind : forall C H T C' H' T', 
+    p_step C H T C' H' T' -> poolRewind C H T ->
+    poolRewind C' H' T'. 
+Proof.
+ intros. induction H0. 
+ {inv H0. econstructor; auto. copy H3. eapply validateValidate in H3.
+  invertHyp. inv H1. eapply rewindNewerStamp. eauto.
+  eapply rewindAbort; eauto. }
+  {inv H0.
+   {inv H1. econstructor; auto. econstructor. 
+    eassumption. econstructor; eauto. }
+   {inv H1. econstructor; auto. econstructor. eassumption.
+    econstructor; eauto. }
+   {inv H1. exfalso; auto. econstructor; eauto.
+    econstructor. eassumption. econstructor; eauto. }
+   {inv H1. exfalso; auto. econstructor; auto.
+    econstructor. eassumption. eapply r_atomicIdemStep; eauto. }
+   {inv H1. exfalso; auto. econstructor; auto.
+    econstructor. eassumption. eapply r_betaStep; eauto. }
+  }
+  {inv H1. econstructor; eauto. eapply p_stepNI; eauto. }
+  {inv H1. econstructor; eauto. eapply p_stepNI; eauto. }
+  {repeat econstructor. }
+  {repeat econstructor. }
+  {econstructor. }
+  {econstructor. econstructor. auto. }
+  {econstructor. }
+  {inv H1. econstructor; auto. eapply rewindNewerStamp; eauto. }
 Qed. 
